Wavelet/Seq/Prog.lean
@@ -4,6 +4,12 @@ import Wavelet.Seq.Fn
 
 /-! Syntax and semantics of programs (a list of `Fn`s with a acyclic call graph). -/
 
+/-- TODO: move this to a better place. -/
+@[simp, grind]
+abbrev Fin.castPred (k' : Fin (k + 1)) (self : Fin ↑k') : Fin k := self.castLT (by omega)
+
+prefix:max " ↓ " => Fin.castPred _
+
 namespace Wavelet.Seq
 
 open Semantics
@@ -12,32 +18,38 @@ structure Sig where
   ι : Nat
   ω : Nat
 
-inductive SigOps (sigs : Vector Sig k) (k' : Fin (k + 1)) where
+abbrev Sigs k := Fin k → Sig
+
+inductive SigOps (sigs : Sigs k) (k' : Fin (k + 1)) where
   | call (i : Fin k')
   deriving DecidableEq
 
 @[simp]
-def SigOps.toFin {k' : Fin (k + 1)} : SigOps sigs k' → Fin k'
+def SigOps.toFin' {sigs : Sigs k} {k' : Fin (k + 1)} : SigOps sigs k' → Fin k'
   | .call i => i
+
+@[simp]
+def SigOps.toFin {sigs : Sigs k} {k' : Fin (k + 1)} : SigOps sigs k' → Fin k
+  | .call i => i.castLT (by omega)
 
 def SigOps.elim0 : SigOps sigs ⟨0, by simp⟩ → α
   | .call i => i.elim0
 
 instance : Arity (SigOps sigs k') where
-  ι | .call i => sigs[i].ι
-  ω | .call i => sigs[i].ω
+  ι | .call i => (sigs ↓i).ι
+  ω | .call i => (sigs ↓i).ω
 
-abbrev Prog (Op : Type u) χ V [Arity Op] (sigs : Vector Sig k) :=
-  (i : Fin k) → Fn (Op ⊕ SigOps sigs i.castSucc) χ V sigs[i].ι sigs[i].ω
+abbrev Prog (Op : Type u) χ V [Arity Op] (sigs : Sigs k) :=
+  (i : Fin k) → Fn (Op ⊕ SigOps sigs i.castSucc) χ V (sigs i).ι (sigs i).ω
 
 /-- Semantics of programs by semantically linking dependent functions. -/
 def Prog.semantics
   [Arity Op] [DecidableEq χ] [InterpConsts V]
-  {sigs : Vector Sig k}
+  {sigs : Sigs k}
   (prog : Prog Op χ V sigs)
   (i : Fin k)
-  : Semantics Op V sigs[i].ι sigs[i].ω
+  : Semantics Op V (sigs i).ι (sigs i).ω
   := Semantics.link (prog i).semantics (λ op =>
-    Prog.semantics prog ⟨op.toFin, by omega⟩)
+    Prog.semantics prog op.toFin)
 
 end Wavelet.Seq
