Wavelet/Typing.lean
@@ -29,15 +29,15 @@ def SimpleIOSpec.toIOSpec (spec : SimpleIOSpec T) m n :
     post _ := spec.post,
   }
 
-abbrev SimpleProgSpec (Op : Type u) T [Arity Op] (_sigs : Vector Sig k) :=
+abbrev SimpleProgSpec (Op : Type u) T [Arity Op] (_sigs : Sigs k) :=
   (i : Fin k) → SimpleIOSpec T
 
 def SimpleProgSpec.toProgSpec
   [Arity Op]
-  {sigs : Vector Sig k}
+  {sigs : Sigs k}
   (spec : SimpleProgSpec Op T sigs) :
     ProgSpec Op V T sigs :=
-  λ i => (spec i).toIOSpec sigs[i].ι sigs[i].ω
+  λ i => (spec i).toIOSpec (sigs i).ι (sigs i).ω
 
 /-- `.inl` for base vars, `.inr` for token variables. -/
 abbrev TypedName χ := χ ⊕ Nat
@@ -135,40 +135,37 @@ def Fn.WellPermTyped
   fn'.params = (fn.params.map .inl).push (.inr 0) ∧
   Expr.WellPermTyped ioSpec (.init (ioSpec.pre)) fn.body fn'.body
 
-def Fn.WellPermTypedDep
-  [Arity Op] [PCM T]
-  {opSpec : OpSpec Op V T}
-  (ioSpec : IOSpec V T m n)
-  (fn : Fn Op χ V m n)
-  (fn' : FnWithSpec opSpec (TypedName χ) m n) :
-  Prop := sorry
+-- def Fn.WellPermTypedDep
+--   [Arity Op] [PCM T]
+--   {opSpec : OpSpec Op V T}
+--   (ioSpec : IOSpec V T m n)
+--   (fn : Fn Op χ V m n)
+--   (fn' : FnWithSpec opSpec (TypedName χ) m n) :
+--   Prop := sorry
 
-def Prog.WellPermTyped
-  [Arity Op] [PCM T]
-  {sigs : Vector Sig k}
-  {opSpec : OpSpec Op V T}
-  {progSpec : ProgSpec Op V T sigs}
-  (prog : Prog Op χ V sigs)
-  (prog' : ProgWithSpecAlt (TypedName χ) opSpec progSpec)
-  (i : Fin k) : Prop
-  := Fn.WellPermTypedDep (progSpec i) (prog i) (prog' i)
+-- def Prog.WellPermTyped
+--   [Arity Op] [PCM T]
+--   {sigs : Sigs k}
+--   {opSpec : OpSpec Op V T}
+--   {progSpec : ProgSpec Op V T sigs}
+--   (prog : Prog Op χ V sigs)
+--   (prog' : ProgWithSpec (TypedName χ) opSpec progSpec)
+--   (i : Fin k) : Prop
+--   := Fn.WellPermTypedDep (progSpec i) (prog i) (prog' i)
 
 -- theorem sim_type_check_prog
---   {Op V T χ : Type 1} -- TODO: relax this constraint
 --   [Arity Op]
 --   [InterpConsts V]
 --   [PCM T] [PCM.Lawful T]
 --   [DecidableEq χ]
 --   [DecidableLE T]
---   {sigs : Vector Sig k}
+--   {sigs : Sigs k}
 --   {opSpec : OpSpec Op V T}
 --   {progSpec : ProgSpec Op V T sigs}
 --   (prog : Prog Op χ V sigs)
---   (prog' : ProgWithSpecAlt (TypedName χ) opSpec progSpec)
---   (hwt : prog.WellPermTyped prog' i) :
---   prog.semantics i ≲
---     ((prog'.toLinkable.semantics i) : Semantics _ _ _ _).guard
---       (opSpec.Guard (progSpec i))
+--   (prog' : ProgWithSpec (TypedName χ) sigs opSpec)
+--   -- (hwt : prog.WellPermTyped prog' i)
+--   : prog.semantics i ≲ (prog'.semantics i).guard (opSpec.Guard (progSpec i))
 --   := by sorry
 
 def SimRel
