Wavelet/HighLevel.lean
@@ -1,0 +1,60 @@
+import Wavelet.Determinacy
+import Wavelet.Seq
+import Wavelet.Dataflow
+import Wavelet.Compile
+import Wavelet.Typing
+
+/-! Some high-level theorems and plans. -/
+
+namespace Wavelet
+
+open Semantics Determinacy Seq Dataflow Compile
+
+/-- TODO -/
+def ProgWithSpec.WellPermTyped
+  [Arity Op] [PCM T]
+  {sigs : Sigs k}
+  {opSpec : OpSpec Op V T}
+  (progSpec : ProgSpec Op V T sigs)
+  (prog : ProgWithSpec χ sigs opSpec) : Prop := sorry
+
+/-- Well-typing induces a simulation between unguarded
+and guarded semantics of `Prog`. -/
+theorem sim_wt_prog
+  [Arity Op]
+  [InterpConsts V]
+  [PCM T] [PCM.Lawful T]
+  [DecidableEq χ]
+  {sigs : Sigs k}
+  {opSpec : OpSpec Op V T}
+  {progSpec : ProgSpec Op V T sigs}
+  (prog : ProgWithSpec χ sigs opSpec)
+  (hwt : ProgWithSpec.WellPermTyped progSpec prog) :
+    (prog.semantics i).guard opSpec.TrivGuard
+      ≲ᵣ (prog.semantics i).guard (opSpec.Guard (progSpec i))
+  := by sorry
+
+theorem compile_forward_sim
+  [Arity Op] [PCM T] [PCM.Lawful T]
+  [DecidableEq χ]
+  [InterpConsts V]
+  {sigs : Sigs k}
+  {opSpec : OpSpec Op V T}
+  {progSpec : ProgSpec Op V T sigs}
+  (prog : ProgWithSpec χ sigs opSpec)
+  (hwt : ProgWithSpec.WellPermTyped progSpec prog)
+  (haff₁ : ∀ (i : Fin k), (prog i).AffineVar)
+  (haff₂ : prog.AffineInrOp)
+  (i : Fin k) :
+    (prog.semantics i).guard opSpec.TrivGuard
+      ≲ᵣ (compileProg _ prog i).semantics.guard opSpec.TrivGuard
+  := by
+  apply IORestrictedSimilarity.trans
+  · exact sim_wt_prog prog hwt
+  apply IORestrictedSimilarity.trans
+  · apply sim_guard
+    apply sim_compile_prog.{_, _, _, 0} (extendSigs sigs) prog ↑i (by omega) haff₁ haff₂
+  simp
+  sorry
+
+end Wavelet
